src/StandardLibrary/StandardLibrary.dfy
@@ -176,8 +176,9 @@ module {:extern "STL"} StandardLibrary {
     a := new T[|s|](i requires 0 <= i < |s| => s[i]);
   }
 
-  lemma SeqPartsMakeWhole<T>(s: seq<T>)
-    ensures forall i :: 0 <= i <= |s| ==> s[..i] + s[i..] == s
+  lemma SeqPartsMakeWhole<T>(s: seq<T>, i: nat)
+    requires 0 <= i <= |s|
+    ensures s[..i] + s[i..] == s
   {}
 
   /*
